state/Examples.HO.fst
@@ -28,7 +28,7 @@ let f_a3p a3p : pck_spec a3p =
               (safe_importable_is_importable a3p unit Leaf).c_styp
               (fun x h0 r h1 -> (Mktuple3?._1 a3p) h1 /\ (Mktuple3?._3 a3p) h0 h1 /\ (Inr? r \/ sel h0 x == sel h1 x)))
 
-let f_spec : pck_spec concrete_spec = f_a3p concrete_spec
+let f_spec : pck_spec c3p = f_a3p c3p
 
 let f_eqx_is_safe_importable a3p : safe_importable_to a3p (f_eqx a3p) (Node (f_a3p a3p) Leaf Leaf) =
   solve
@@ -39,7 +39,7 @@ let f_eqx_is_safe_importable a3p : safe_importable_to a3p (f_eqx a3p) (Node (f_a
     (fun x h0 -> (Mktuple3?._1 a3p) h0 /\ satisfy x (prref_c))
     (fun x h0 r h1 -> (Mktuple3?._1 a3p) h1 /\ (Mktuple3?._3 a3p) h0 h1 /\ (Inr? r \/ sel h0 x == sel h1 x))**)
 
-let f_hoc : hoc concrete_spec f_spec =
+let f_hoc : hoc c3p f_spec =
 EnforcePost
     (fun _ -> ())
     (fun _ _ -> ())
@@ -48,11 +48,11 @@ EnforcePost
       recall (contains_pred rx);
       let x = sst_read rx in
       let eh0 = get_heap () in
-      let check : cb_check concrete_spec (ref int) (resexn unit) (fun x -> sst_pre (fun h0 -> satisfy x (prref_c))) (fun x -> sst_post _ _ (fun h0 r h1 -> Inr? r \/ sel h0 x == sel h1 x)) rx eh0 =
+      let check : cb_check c3p (ref int) (resexn unit) (fun x -> sst_pre (fun h0 -> satisfy x (prref_c))) (fun x -> sst_post _ _ (fun h0 r h1 -> Inr? r \/ sel h0 x == sel h1 x)) rx eh0 =
         (fun kres -> if x = sst_read rx then Inl () else Inr (Contract_failure "x has changed")) in
       (| eh0, check |))
 
-let f_pkhoc : pck_hoc concrete_spec =
+let f_pkhoc : pck_hoc c3p =
   (| f_spec, f_hoc |)
 
 let f_tree : hoc_tree (Node f_spec Leaf Leaf) =
@@ -75,7 +75,7 @@ let unsafe_f x =
   Inl ()**)
 
 val tgt_f : ctx_tgt1 (comp_int_src_tgt1 sit)
-let tgt_f inv prref hrel read write alloc x =
+let tgt_f read write alloc x =
   write x 0;
   Inl ()
 
